Cleanup. Change find_block to a definition instead of fixpoint.
Fixpoint was gross in proofs :(.

src/coq/CFG.v
@@ -116,7 +116,7 @@ Definition blk_entry_pc (fid:function_id) (b:block T) :=
 Definition blk_term_pc (fid:function_id) (b:block T) :=
   mk_pc fid (blk_id b) (blk_term_id b).
 
-Fixpoint find_block bs block_id : option (block T) :=
+Definition find_block bs block_id : option (block T) :=
   find (fun b => if (blk_id b) ~=? block_id then true else false) bs.
 
 Fixpoint find_instr (cd : (code T)) (p:instr_id) (t:instr_id) : option (cmd * option instr_id) :=
